Remove explicit specification, allow for more general form

Interference.thy
@@ -1,8 +1,8 @@
 theory Interference
-  imports Execution
+  imports Semantics
 begin
 
-locale interference = execution re fwd eval
+locale interference = semantics re fwd eval
   for re :: "'a \<Rightarrow> 'a \<Rightarrow> bool" (infix "\<hookleftarrow>" 100)
   and fwd :: "'a \<Rightarrow> 'a \<Rightarrow> 'a" ("_\<langle>_\<rangle>" [1000,0] 1000)
   and eval :: "'a \<Rightarrow> 's rel"
@@ -16,21 +16,18 @@ text \<open>Independence of two instructions \<beta> and \<alpha> under environm
       such that the early execution of \<alpha> is assumed to be possible and 
       cannot invalidate sequential reasoning\<close>
 definition inter\<^sub>a
-  where "inter\<^sub>a R G X \<beta> \<alpha> \<equiv> 
-          (X \<beta> \<inter> wp \<beta> (st R (X \<alpha>)) \<subseteq> X \<alpha>\<langle>\<beta>\<rangle> \<inter> wp \<alpha>\<langle>\<beta>\<rangle> (st R (X \<beta>)) \<and> 
-          (eval \<alpha>\<langle>\<beta>\<rangle> \<otimes> R\<^sup>* \<otimes> eval \<beta> \<subseteq> eval \<beta> \<otimes> R\<^sup>* \<otimes> eval \<alpha>)) \<and>
-          (X \<alpha>\<langle>\<beta>\<rangle> \<subseteq> spec \<alpha>\<langle>\<beta>\<rangle> G)"
+  where "inter\<^sub>a R G \<beta> \<alpha> \<equiv> R\<^sup>* \<otimes> eval \<alpha>\<langle>\<beta>\<rangle> \<otimes> R\<^sup>* \<otimes> eval \<beta> \<subseteq> R\<^sup>* \<otimes> eval \<beta> \<otimes> R\<^sup>* \<otimes> eval \<alpha> \<and> spec \<alpha>\<langle>\<beta>\<rangle> G"
 
 text \<open>Independence of program c and instruction \<alpha> under environment R, 
       such that the early execution of \<alpha> is assumed to be possible and 
       cannot invalidate sequential reasoning\<close>
 fun inter\<^sub>c
   where
-    "inter\<^sub>c R G X (Basic \<beta>) \<alpha> = inter\<^sub>a R G X \<beta> \<alpha>" |
-    "inter\<^sub>c R G X (c\<^sub>1 ; c\<^sub>2) \<alpha> = (inter\<^sub>c R G X c\<^sub>1 \<alpha>\<llangle>c\<^sub>2\<rrangle> \<and> inter\<^sub>c R G X c\<^sub>2 \<alpha>)" |
-    "inter\<^sub>c R G X (c\<^sub>1 \<sqinter> c\<^sub>2) \<alpha> = (inter\<^sub>c R G X c\<^sub>1 \<alpha> \<and> inter\<^sub>c R G X c\<^sub>2 \<alpha>)" |
-    "inter\<^sub>c R G X (c*) \<alpha> = inter\<^sub>c R G X c \<alpha>" |
-    "inter\<^sub>c R G X _ \<alpha> = True"
+    "inter\<^sub>c R G (Basic \<beta>) \<alpha> = inter\<^sub>a R G \<beta> \<alpha>" |
+    "inter\<^sub>c R G (c\<^sub>1 ; c\<^sub>2) \<alpha> = (inter\<^sub>c R G c\<^sub>1 \<alpha>\<llangle>c\<^sub>2\<rrangle> \<and> inter\<^sub>c R G c\<^sub>2 \<alpha>)" |
+    "inter\<^sub>c R G (c\<^sub>1 \<sqinter> c\<^sub>2) \<alpha> = (inter\<^sub>c R G c\<^sub>1 \<alpha> \<and> inter\<^sub>c R G c\<^sub>2 \<alpha>)" |
+    "inter\<^sub>c R G (c*) \<alpha> = inter\<^sub>c R G c \<alpha>" |
+    "inter\<^sub>c R G _ \<alpha> = True"
 
 text \<open>Instrumented version of the semantics that collects the reordering effects\<close>
 inductive_set execute_collect :: "('a com \<times> 'a \<times> 'a com \<times> 'a \<times> 'a com) set"
@@ -43,24 +40,29 @@ inductive_set execute_collect :: "('a com \<times> 'a \<times> 'a com \<times> '
   pst[intro]:  "c\<^sub>1 \<mapsto>[\<alpha>,c,\<alpha>'] c\<^sub>1' \<Longrightarrow> \<gamma> < c\<^sub>2 <\<^sub>p \<alpha> \<Longrightarrow> c\<^sub>2 ; c\<^sub>1 \<mapsto>[\<gamma>,c\<^sub>2;c,\<alpha>'] c\<^sub>2 ; c\<^sub>1'"
 inductive_cases execute_collect[elim]: "c\<^sub>1 \<mapsto>[\<alpha>,c,\<alpha>'] c\<^sub>1'"
 
-text \<open>Interference property preserved throughout execution\<close>
-inductive inter
-  where "(\<forall>c' \<alpha> \<alpha>' r. c \<mapsto>[\<alpha>,r,\<alpha>'] c' \<longrightarrow> (inter R G X c' \<and> inter\<^sub>c R G X r \<alpha>')) \<Longrightarrow> 
-         (\<forall>c'. c \<leadsto> c' \<longrightarrow> inter R G X c') \<Longrightarrow> inter R G X c"
+text \<open>Compute possible reorderings of the program using the instrumented semantics\<close>
+inductive reorder_trace
+  where 
+    "reorder_trace [] c" |
+    "c \<leadsto> c' \<Longrightarrow> reorder_trace t c' \<Longrightarrow> reorder_trace t c" |
+    "c \<mapsto>[\<alpha>,r,\<alpha>'] c' \<Longrightarrow> reorder_trace t c' \<Longrightarrow> reorder_trace ((r,\<alpha>')#t) c"
+
+text \<open>Ensure all reorderings enforce the necessary interference property\<close>
+definition inter
+  where "inter R G c \<equiv> \<forall>t. reorder_trace t c \<longrightarrow> (\<forall>(r,\<alpha>) \<in> set t. inter\<^sub>c R G r \<alpha>)"
 
 text \<open>Interference is preserved across a silent step\<close>
 lemma inter_silentI [intro]:
-  assumes "inter R G X c" "c \<leadsto> c'"
-  shows "inter R G X c'"
-  using assms 
-  by cases auto
+  assumes "inter R G c" "c \<leadsto> c'"
+  shows "inter R G c'"
+  using assms by (auto simp: inter_def intro: reorder_trace.intros)
 
 text \<open>Interference is preserved across an execution step and prevents interference\<close>
 lemma indep_stepI [intro]:
-  assumes "inter R G X c" "c \<mapsto>[\<alpha>,r,\<alpha>'] c'"
-  shows "inter R G X c' \<and> inter\<^sub>c R G X r \<alpha>'"
-  using assms 
-  by cases auto
+  assumes "inter R G c" "c \<mapsto>[\<alpha>,r,\<alpha>'] c'"
+  shows "inter R G c' \<and> inter\<^sub>c R G r \<alpha>'"
+  using assms reorder_trace.intros(1,3)
+  unfolding inter_def by force
 
 text \<open>Instrumented semantics collects valid reorderings\<close>
 lemma collect_reorder:
