Local_Rules.thy
@@ -1,12 +1,10 @@
 theory Local_Rules
-  imports Execution
+  imports Semantics
 begin
 
 chapter \<open>Thread Local Rules\<close>
 
-type_synonym ('a,'s) ctxs = "'a \<Rightarrow> 's set"
-
-locale local_rules = execution re fwd eval
+locale local_rules = semantics re fwd eval
   for re :: "'a \<Rightarrow> 'a \<Rightarrow> bool" (infix "\<hookleftarrow>" 100)
   and fwd :: "'a \<Rightarrow> 'a \<Rightarrow> 'a" ("_\<langle>_\<rangle>" [1000,0] 1000)
   and eval :: "'a \<Rightarrow> 's rel"
@@ -21,20 +19,20 @@ definition stable
   where "stable R P \<equiv> \<forall>m m'. m \<in> P \<longrightarrow> (m,m') \<in> R \<longrightarrow> m' \<in> P"
 
 text \<open>Rule for an atomic operation with a context\<close>
-definition atomic_rule :: "'s rel \<Rightarrow> 's rel \<Rightarrow> ('a,'s) ctxs \<Rightarrow> 's set \<Rightarrow> 'a \<Rightarrow> 's set \<Rightarrow> bool" 
-  ("_,_,_ \<turnstile>\<^sub>A _ {_} _" [20, 20, 20, 20] 20)
-  where "R,G,X \<turnstile>\<^sub>A P {\<alpha>} Q \<equiv> P \<subseteq> wp \<alpha> Q \<inter> X \<alpha> \<and> X \<alpha> \<subseteq> spec \<alpha> G \<and> stable R P \<and> stable R Q"
+definition atomic_rule :: "'s rel \<Rightarrow> 's rel \<Rightarrow> 's set \<Rightarrow> 'a \<Rightarrow> 's set \<Rightarrow> bool" 
+  ("_,_ \<turnstile>\<^sub>A _ {_} _" [20, 20, 20, 20] 20)
+  where "R,G \<turnstile>\<^sub>A P {\<alpha>} Q \<equiv> P \<subseteq> wp \<alpha> Q \<and> spec \<alpha> G \<and> stable R P \<and> stable R Q"
 
 text \<open>Establish the rules of the logic, similar to standard Hoare-logic\<close>
-inductive lrules :: "'s rel \<Rightarrow> 's rel \<Rightarrow> ('a,'s) ctxs \<Rightarrow> 's set \<Rightarrow> 'a com \<Rightarrow> 's set \<Rightarrow> bool"
-  ("_,_,_ \<turnstile>\<^sub>t _ {_} _" [20,0,0,0,20] 20)
+inductive lrules :: "'s rel \<Rightarrow> 's rel \<Rightarrow> 's set \<Rightarrow> 'a com \<Rightarrow> 's set \<Rightarrow> bool"
+  ("_,_ \<turnstile>\<^sub>t _ {_} _" [20,0,0,0,20] 20)
 where
-  nil[intro]:    "stable R P \<Longrightarrow> R,G,X \<turnstile>\<^sub>t P { Nil } P" |
-  seq[intro]:    "R,G,X \<turnstile>\<^sub>t P { c\<^sub>1 } Q \<Longrightarrow> R,G,X \<turnstile>\<^sub>t Q { c\<^sub>2 } M \<Longrightarrow> R,G,X \<turnstile>\<^sub>t P { c\<^sub>1 ; c\<^sub>2 } M" |
-  choice[intro]: "R,G,X \<turnstile>\<^sub>t P { c\<^sub>1 } Q \<Longrightarrow> R,G,X \<turnstile>\<^sub>t P { c\<^sub>2 } Q \<Longrightarrow> R,G,X \<turnstile>\<^sub>t P { c\<^sub>1 \<sqinter> c\<^sub>2 } Q" |
-  loop[intro]:   "stable R P \<Longrightarrow> R,G,X \<turnstile>\<^sub>t P { c } P \<Longrightarrow> R,G,X \<turnstile>\<^sub>t P { c* } P" |
-  basic[intro]:  "R,G,X \<turnstile>\<^sub>A P {\<alpha>} Q \<Longrightarrow> R,G,X \<turnstile>\<^sub>t P { Basic \<alpha> } Q" |
-  conseq[intro]: "R,G,X \<turnstile>\<^sub>t P { c } Q \<Longrightarrow> P' \<subseteq> P \<Longrightarrow> R' \<subseteq> R \<Longrightarrow> G \<subseteq> G' \<Longrightarrow> Q \<subseteq> Q' \<Longrightarrow> R',G',X \<turnstile>\<^sub>t P' { c } Q'"
+  nil[intro]:    "stable R P \<Longrightarrow> R,G \<turnstile>\<^sub>t P { Nil } P" |
+  seq[intro]:    "R,G \<turnstile>\<^sub>t P { c\<^sub>1 } Q \<Longrightarrow> R,G \<turnstile>\<^sub>t Q { c\<^sub>2 } M \<Longrightarrow> R,G \<turnstile>\<^sub>t P { c\<^sub>1 ; c\<^sub>2 } M" |
+  choice[intro]: "R,G \<turnstile>\<^sub>t P { c\<^sub>1 } Q \<Longrightarrow> R,G \<turnstile>\<^sub>t P { c\<^sub>2 } Q \<Longrightarrow> R,G \<turnstile>\<^sub>t P { c\<^sub>1 \<sqinter> c\<^sub>2 } Q" |
+  loop[intro]:   "stable R P \<Longrightarrow> R,G \<turnstile>\<^sub>t P { c } P \<Longrightarrow> R,G \<turnstile>\<^sub>t P { c* } P" |
+  basic[intro]:  "R,G \<turnstile>\<^sub>A P {\<alpha>} Q \<Longrightarrow> R,G \<turnstile>\<^sub>t P { Basic \<alpha> } Q" |
+  conseq[intro]: "R,G \<turnstile>\<^sub>t P { c } Q \<Longrightarrow> P' \<subseteq> P \<Longrightarrow> R' \<subseteq> R \<Longrightarrow> G \<subseteq> G' \<Longrightarrow> Q \<subseteq> Q' \<Longrightarrow> R',G' \<turnstile>\<^sub>t P' { c } Q'"
 
 section \<open>Helper Lemmas\<close>
 
@@ -49,39 +47,39 @@ lemma stable_conjI [intro]:
   using assms by (auto simp: stable_def)
 
 lemma spec_conseqI [intro]:
-  assumes "G' \<subseteq> G" 
-  shows "spec \<alpha> G' \<subseteq> spec \<alpha> G"
+  assumes "G' \<subseteq> G" "spec \<alpha> G'"
+  shows "spec \<alpha> G"
   using assms unfolding spec_def by auto
 
 lemma thread_only:
-  assumes "R,G,X \<turnstile>\<^sub>t P { c } Q"
+  assumes "R,G \<turnstile>\<^sub>t P { c } Q"
   shows "local_only c"
   using assms by induct auto
 
 section \<open>Atomic Rules\<close>
 
 lemma atomic_pre:
-  assumes "R,G,X \<turnstile>\<^sub>A P {\<alpha>} Q" "P' \<subseteq> P" "stable R P'"
-  shows "R,G,X \<turnstile>\<^sub>A P' {\<alpha>} Q"
+  assumes "R,G \<turnstile>\<^sub>A P {\<alpha>} Q" "P' \<subseteq> P" "stable R P'"
+  shows "R,G \<turnstile>\<^sub>A P' {\<alpha>} Q"
   using assms unfolding atomic_rule_def
   by fast
 
 lemma atomic_conseqI [intro]:
-  assumes "R,G,X \<turnstile>\<^sub>A P {\<alpha>} Q" "R' \<subseteq> R" "G \<subseteq> G'"
-  shows "R',G',X \<turnstile>\<^sub>A P {\<alpha>} Q"
+  assumes "R,G \<turnstile>\<^sub>A P {\<alpha>} Q" "R' \<subseteq> R" "G \<subseteq> G'"
+  shows "R',G' \<turnstile>\<^sub>A P {\<alpha>} Q"
   using assms spec_conseqI unfolding atomic_rule_def
   by blast
 
 lemma actomic_conjI [intro]:
-  assumes "R,G,X \<turnstile>\<^sub>A P\<^sub>1 {\<alpha>} Q\<^sub>1" "R,G,X  \<turnstile>\<^sub>A P\<^sub>2 {\<alpha>} Q\<^sub>2"
-  shows "R,G,X \<turnstile>\<^sub>A (P\<^sub>1 \<inter> P\<^sub>2) {\<alpha>} (Q\<^sub>1 \<inter> Q\<^sub>2)"
+  assumes "R,G \<turnstile>\<^sub>A P\<^sub>1 {\<alpha>} Q\<^sub>1" "R,G  \<turnstile>\<^sub>A P\<^sub>2 {\<alpha>} Q\<^sub>2"
+  shows "R,G \<turnstile>\<^sub>A (P\<^sub>1 \<inter> P\<^sub>2) {\<alpha>} (Q\<^sub>1 \<inter> Q\<^sub>2)"
   using assms unfolding atomic_rule_def  
   by (auto simp: wp_def stable_def)
 
 lemma atomic_frameI [intro]:
-  assumes "R,G,X \<turnstile>\<^sub>A P {\<alpha>} Q"
+  assumes "R,G \<turnstile>\<^sub>A P {\<alpha>} Q"
   assumes "stable R\<^sub>2 M" "G \<subseteq> R\<^sub>2"
-  shows "R \<inter> R\<^sub>2,G,X \<turnstile>\<^sub>A P \<inter> M {\<alpha>} Q \<inter> M"
+  shows "R \<inter> R\<^sub>2,G \<turnstile>\<^sub>A P \<inter> M {\<alpha>} Q \<inter> M"
   unfolding atomic_rule_def
 proof (safe, goal_cases)
   case (1 x)
@@ -95,63 +93,63 @@ qed (insert assms, auto simp: atomic_rule_def wp_def)
 section \<open>Elimination Rules\<close>
 
 lemma nilE [elim!]:
-  assumes "R,G,X \<turnstile>\<^sub>t P {Nil} Q"
+  assumes "R,G \<turnstile>\<^sub>t P {Nil} Q"
   obtains M where "stable R M" "P \<subseteq> M" "M \<subseteq> Q"
-  using assms by (induct R G X P "Nil :: 'a com" Q) blast+
+  using assms by (induct R G P "Nil :: 'a com" Q) blast+
 
 lemma basicE [elim!]:
-  assumes "R,G,X \<turnstile>\<^sub>t P {Basic \<beta>} Q"
-  obtains P' Q' where "P \<subseteq> P'" "R,G,X \<turnstile>\<^sub>A P' {\<beta>} Q'" "Q' \<subseteq> Q"
+  assumes "R,G \<turnstile>\<^sub>t P {Basic \<beta>} Q"
+  obtains P' Q' where "P \<subseteq> P'" "R,G \<turnstile>\<^sub>A P' {\<beta>} Q'" "Q' \<subseteq> Q"
   using assms 
-proof (induct R G X P "Basic \<beta>" Q)
-  case (basic R G X P Q)
+proof (induct R G P "Basic \<beta>" Q)
+  case (basic R G P Q)
   then show ?case by auto
 next
-  case (conseq R G X P Q P' R' G' Q')
+  case (conseq R G P Q P' R' G' Q')
   then show ?case using order.trans atomic_conseqI by metis
 qed
 
 lemma seqE [elim]:
-  assumes "R,G,X \<turnstile>\<^sub>t P {c\<^sub>1 ; c\<^sub>2} Q"
-  obtains M  where "R,G,X \<turnstile>\<^sub>t P {c\<^sub>1} M" "R,G,X \<turnstile>\<^sub>t M {c\<^sub>2} Q"
+  assumes "R,G \<turnstile>\<^sub>t P {c\<^sub>1 ; c\<^sub>2} Q"
+  obtains M  where "R,G \<turnstile>\<^sub>t P {c\<^sub>1} M" "R,G \<turnstile>\<^sub>t M {c\<^sub>2} Q"
   using assms 
-  by (induct R G X P "c\<^sub>1 ; c\<^sub>2" Q arbitrary: c\<^sub>1 c\<^sub>2) blast+
+  by (induct R G P "c\<^sub>1 ; c\<^sub>2" Q arbitrary: c\<^sub>1 c\<^sub>2) blast+
 
 lemma choiceE [elim]:
-  assumes "R,G,X \<turnstile>\<^sub>t P {c\<^sub>1 \<sqinter> c\<^sub>2} Q"
-  obtains "R,G,X \<turnstile>\<^sub>t P {c\<^sub>1} Q" "R,G,X \<turnstile>\<^sub>t P {c\<^sub>2} Q"
-  using assms by (induct R G X P "c\<^sub>1 \<sqinter> c\<^sub>2" Q arbitrary: c\<^sub>1 c\<^sub>2) auto
+  assumes "R,G \<turnstile>\<^sub>t P {c\<^sub>1 \<sqinter> c\<^sub>2} Q"
+  obtains "R,G \<turnstile>\<^sub>t P {c\<^sub>1} Q" "R,G \<turnstile>\<^sub>t P {c\<^sub>2} Q"
+  using assms by (induct R G P "c\<^sub>1 \<sqinter> c\<^sub>2" Q arbitrary: c\<^sub>1 c\<^sub>2) auto
 
 lemma loopE [elim]:
-  assumes "R,G,X \<turnstile>\<^sub>t P { c* } Q"
-  obtains I where "P \<subseteq> I" "R,G,X \<turnstile>\<^sub>t I { c } I" "I \<subseteq> Q" "stable R I"
+  assumes "R,G \<turnstile>\<^sub>t P { c* } Q"
+  obtains I where "P \<subseteq> I" "R,G \<turnstile>\<^sub>t I { c } I" "I \<subseteq> Q" "stable R I"
   using assms 
-proof (induct R G X P "c*" Q arbitrary: c)
+proof (induct R G P "c*" Q arbitrary: c)
   case (loop R G P c)
   then show ?case by blast
 next
-  case (conseq R G X P Q P' R' G' Q')
+  case (conseq R G P Q P' R' G' Q')
   then show ?case using lrules.conseq stable_conseqI by (metis subset_eq)
 qed
 
 lemma parE [elim!]:
-  assumes "R,G,X \<turnstile>\<^sub>t P { c\<^sub>1 || c\<^sub>2 } Q"
+  assumes "R,G \<turnstile>\<^sub>t P { c\<^sub>1 || c\<^sub>2 } Q"
   obtains "False"
   using assms 
-proof (induct R G X P "c\<^sub>1 || c\<^sub>2" Q)
-  case (conseq R G X P Q P' R' G' Q')
+proof (induct R G P "c\<^sub>1 || c\<^sub>2" Q)
+  case (conseq R G P Q P' R' G' Q')
   thus ?case by blast
 qed
 
 lemma stable_preE:
-  assumes "R,G,X \<turnstile>\<^sub>t P {c} Q"
-  obtains P' where "P \<subseteq> P'" "stable R P'" "R,G,X \<turnstile>\<^sub>t P' {c} Q"
+  assumes "R,G \<turnstile>\<^sub>t P {c} Q"
+  obtains P' where "P \<subseteq> P'" "stable R P'" "R,G \<turnstile>\<^sub>t P' {c} Q"
   using assms 
 proof (induct)
-  case (basic R G X P \<alpha> Q)
+  case (basic R G P \<alpha> Q)
   then show ?case using atomic_rule_def by fast
 next
-  case (choice R G X P c\<^sub>1 Q c\<^sub>2)
+  case (choice R G P c\<^sub>1 Q c\<^sub>2)
   show ?case
   proof (rule choice(2), rule choice(4),  goal_cases)
     case (1 P' P'')
