Soundness.thy
@@ -72,13 +72,13 @@ lemma stable_stI [intro]:
   using assms stable_transitive by (auto simp: st_def)
 
 lemma atomic_strongest:
-  assumes "R,G,X \<turnstile>\<^sub>A P {\<alpha>} Q"
-  shows "(R,G,X \<turnstile>\<^sub>A P {\<alpha>} (sp \<alpha> R P)) \<and> sp \<alpha> R P \<subseteq> Q"
+  assumes "R,G \<turnstile>\<^sub>A P {\<alpha>} Q"
+  shows "(R,G \<turnstile>\<^sub>A P {\<alpha>} (sp \<alpha> R P)) \<and> sp \<alpha> R P \<subseteq> Q"
 proof -
   have "Q \<subseteq> st R Q" "P \<subseteq> wp \<alpha> Q" 
     using assms stable_transitive unfolding atomic_rule_def st_def wp_def by fast+
   hence "sp \<alpha> R P \<subseteq> Q" by (auto simp: sp_def wp_def st_def)
-  moreover have "R,G,X \<turnstile>\<^sub>A P {\<alpha>} (sp \<alpha> R P)"
+  moreover have "R,G \<turnstile>\<^sub>A P {\<alpha>} (sp \<alpha> R P)"
     using assms by (clarsimp simp add: atomic_rule_def wp_def stable_def sp_def) force
   ultimately show ?thesis by auto
 qed
@@ -88,52 +88,41 @@ text \<open>
   The precondition P and postcondition Q are preserved.
 \<close>
 lemma reorder_action:
-  assumes "R,G,X \<turnstile>\<^sub>A P {\<beta>} M" "R,G,X \<turnstile>\<^sub>A M {\<alpha>} Q" "\<beta> \<hookleftarrow> fwd \<alpha> \<beta>" "inter\<^sub>a R G X \<beta> \<alpha>"
-  obtains M' where "R,G,X \<turnstile>\<^sub>A P {fwd \<alpha> \<beta>} M'" "R,G,X \<turnstile>\<^sub>A M' {\<beta>} Q"
+  assumes "R,G \<turnstile>\<^sub>A P {\<beta>} M" "R,G \<turnstile>\<^sub>A M {\<alpha>} Q" "\<beta> \<hookleftarrow> fwd \<alpha> \<beta>" "inter\<^sub>a R G \<beta> \<alpha>"
+  obtains M' where "R,G \<turnstile>\<^sub>A P {fwd \<alpha> \<beta>} M'" "R,G \<turnstile>\<^sub>A M' {\<beta>} Q"
 proof -
-  \<comment> \<open>Nominate the weakest-precondition of \<beta> over Q as the state between the new \<alpha> and \<beta>\<close>
+  \<comment> \<open>Nominate the strongest-postcondition of \<alpha> from P as the state between \<alpha> and \<beta>\<close>
   let ?\<alpha>="fwd \<alpha> \<beta>"
   let ?M="sp ?\<alpha> R P"
 
   \<comment> \<open>Extract order independence properties\<close>
-  have inter: "X \<beta> \<inter> wp \<beta> (st R (X \<alpha>)) \<subseteq> X ?\<alpha> \<inter> wp ?\<alpha> (st R (X \<beta>))"
+  have "R\<^sup>* \<otimes> eval ?\<alpha> \<otimes> R\<^sup>* \<otimes> eval \<beta> \<subseteq> R\<^sup>* \<otimes> eval \<beta> \<otimes> R\<^sup>* \<otimes> eval \<alpha>"
     using assms(4) by (auto simp: inter\<^sub>a_def)
-  have "eval ?\<alpha> \<otimes> R\<^sup>* \<otimes> eval \<beta> \<subseteq> eval \<beta> \<otimes> R\<^sup>* \<otimes> eval \<alpha>"
-    using assms(4) by (auto simp: inter\<^sub>a_def)
-  hence env: "\<forall>Q. st R (wp \<beta> (st R (wp \<alpha> (st R Q)))) \<subseteq> wp ?\<alpha> (st R (wp \<beta> Q))"
+  hence env: "\<forall>Q. st R (wp \<beta> (st R (wp \<alpha> Q))) \<subseteq> st R (wp ?\<alpha> (st R (wp \<beta> Q)))"
     unfolding comp_def wp_def st_def by safe blast 
-  have g: "X ?\<alpha> \<subseteq> spec ?\<alpha> G" using assms(4) by (auto simp: inter\<^sub>a_def)
+  have g: "spec ?\<alpha> G" using assms(4) by (auto simp: inter\<^sub>a_def)
 
-  \<comment> \<open>Extract stability for P, Q and the new intermediate state\<close>
-  have stablePQ: "stable R P" "stable R Q" "X \<alpha> \<subseteq> spec \<alpha> G" "X \<beta> \<subseteq> spec \<beta> G"
+  \<comment> \<open>Establish stability for P, Q and the new intermediate state, in addition to guarantees\<close>
+  have stablePQ: "stable R P" "stable R Q" "spec \<alpha> G" "spec \<beta> G"
     using assms(1,2) by (auto simp: atomic_rule_def)
   have stableM: "stable R ?M"  unfolding stable_def sp_def by force
 
   \<comment> \<open>Show transition from P to Q is independent of order\<close>
   have p: "P \<subseteq> wp \<beta> M" "M \<subseteq> wp \<alpha> Q" "M \<subseteq> st R M" "P \<subseteq> st R P" "Q \<subseteq> st R Q"
     using assms(1,2) stable_stI unfolding atomic_rule_def wp_def by auto
-  hence "P \<subseteq> st R (wp \<beta> (st R (wp \<alpha> (st R Q))))" unfolding st_def wp_def by blast
-  hence exec: "P \<subseteq> wp ?\<alpha> (st R (wp \<beta> Q))" using env by blast
-
-  \<comment> \<open>Show the contexts for both operations hold under P\<close>
-  have "P \<subseteq> X \<beta> \<inter> wp \<beta> (st R (X \<alpha>))" using assms(1,2) p(3) 
-    unfolding atomic_rule_def wp_def st_def by blast 
-  hence ctx: "P \<subseteq> X ?\<alpha> \<inter> wp ?\<alpha> (st R (X \<beta>))" using inter by blast
+  hence "P \<subseteq> st R (wp \<beta> (st R (wp \<alpha> Q)))" unfolding st_def wp_def by blast
+  hence exec: "P \<subseteq> st R (wp ?\<alpha> (st R (wp \<beta> Q)))" using env by blast
 
   \<comment> \<open>Establish the late judgement over \<beta>\<close>
-  have "R,G,X \<turnstile>\<^sub>A ?M {\<beta>} Q" 
+  have "R,G \<turnstile>\<^sub>A ?M {\<beta>} Q" 
   proof (unfold atomic_rule_def, intro conjI Int_greatest)
     show "?M \<subseteq> wp \<beta> Q" using exec unfolding st_def wp_def sp_def by blast
-  next
-    show "?M \<subseteq> X \<beta>" using ctx unfolding st_def wp_def sp_def by blast
   qed (insert stablePQ stableM, simp)
 
   \<comment> \<open>Establish the early judgement over the new \<alpha>\<close>
-  moreover have "R,G,X \<turnstile>\<^sub>A P {?\<alpha>} ?M"
+  moreover have "R,G \<turnstile>\<^sub>A P {?\<alpha>} ?M"
   proof (unfold atomic_rule_def, intro conjI Int_greatest)
     show "P \<subseteq> wp ?\<alpha> ?M" unfolding wp_def wf_def sp_def by blast
-  next
-    show "P \<subseteq> X (fwd \<alpha> \<beta>)" using ctx by blast
   qed (insert stablePQ stableM g, simp)
 
   ultimately show ?thesis using that by blast
@@ -144,32 +133,32 @@ text \<open>
   interference property.
 \<close>
 lemma reorder_prog:
-  assumes "R,G,X \<turnstile>\<^sub>t P {c} M" "R,G,X \<turnstile>\<^sub>A M {\<alpha>} Q" "\<alpha>' < c <\<^sub>p \<alpha>" "inter\<^sub>c R G X c \<alpha>"
-  obtains M' P' where "P \<subseteq> P'" "R,G,X \<turnstile>\<^sub>A P' {\<alpha>'} M'" "R,G,X \<turnstile>\<^sub>t M' {c} Q"
+  assumes "R,G \<turnstile>\<^sub>t P {c} M" "R,G \<turnstile>\<^sub>A M {\<alpha>} Q" "\<alpha>' < c <\<^sub>p \<alpha>" "inter\<^sub>c R G c \<alpha>"
+  obtains M' P' where "P \<subseteq> P'" "R,G \<turnstile>\<^sub>A P' {\<alpha>'} M'" "R,G \<turnstile>\<^sub>t M' {c} Q"
   using assms
-proof (induct c arbitrary: R G X P M Q \<alpha>' \<alpha>)
+proof (induct c arbitrary: R G P M Q \<alpha>' \<alpha>)
   case Nil
   hence "P \<subseteq> M" by blast
   then show ?case using Nil by (auto simp: atomic_rule_def)
 next
   case (Basic \<beta>)
   have \<alpha>: "\<beta> \<hookleftarrow> \<alpha>\<langle>\<beta>\<rangle>" "\<alpha>' = \<alpha>\<langle>\<beta>\<rangle>" using Basic by auto
-  obtain P' N' where \<beta>: "P \<subseteq> P'" "R,G,X \<turnstile>\<^sub>A P' {\<beta>} N'" "N' \<subseteq> M" using Basic by auto
-  have m': "R,G,X \<turnstile>\<^sub>A N' {\<alpha>} Q"
+  obtain P' N' where \<beta>: "P \<subseteq> P'" "R,G \<turnstile>\<^sub>A P' {\<beta>} N'" "N' \<subseteq> M" using Basic by auto
+  have m': "R,G \<turnstile>\<^sub>A N' {\<alpha>} Q"
     using atomic_pre[OF Basic(3)] \<beta>(2,3) Basic(3) by (auto simp: atomic_rule_def)
-  obtain M' where m'': "R,G,X \<turnstile>\<^sub>A P' {\<alpha>\<langle>\<beta>\<rangle>} M'" "R,G,X \<turnstile>\<^sub>A M' {\<beta>} Q"
+  obtain M' where m'': "R,G \<turnstile>\<^sub>A P' {\<alpha>\<langle>\<beta>\<rangle>} M'" "R,G \<turnstile>\<^sub>A M' {\<beta>} Q"
     using reorder_action[OF \<beta>(2) m'(1) \<alpha>(1)] Basic by auto
-  have "R,G,X \<turnstile>\<^sub>t M' {Basic \<beta>} Q" by (rule lrules.basic[OF m''(2)])
+  have "R,G \<turnstile>\<^sub>t M' {Basic \<beta>} Q" by (rule lrules.basic[OF m''(2)])
   then show ?case using Basic(1) \<beta>(1) m''(1) \<alpha>(2) by auto
 next
   case (Seq c\<^sub>1 c\<^sub>2)
   obtain \<alpha>\<^sub>n where \<alpha>: "\<alpha>' < c\<^sub>1 <\<^sub>p \<alpha>\<^sub>n" "\<alpha>\<^sub>n < c\<^sub>2 <\<^sub>p \<alpha>" using Seq by auto
-  obtain M' where m: "R,G,X \<turnstile>\<^sub>t P {c\<^sub>1} M'" "R,G,X \<turnstile>\<^sub>t M' {c\<^sub>2} M" using Seq(4) by fast
-  have i: "inter\<^sub>c R G X c\<^sub>1 \<alpha>\<^sub>n" "inter\<^sub>c R G X c\<^sub>2 \<alpha>" using Seq \<alpha> by auto
+  obtain M' where m: "R,G \<turnstile>\<^sub>t P {c\<^sub>1} M'" "R,G \<turnstile>\<^sub>t M' {c\<^sub>2} M" using Seq(4) by fast
+  have i: "inter\<^sub>c R G c\<^sub>1 \<alpha>\<^sub>n" "inter\<^sub>c R G c\<^sub>2 \<alpha>" using Seq \<alpha> by auto
   show ?case
   proof (rule Seq(2)[OF _ m(2) Seq(5) \<alpha>(2) i(2)], goal_cases outer)
     case (outer P' N')
-    hence c1: "R,G,X \<turnstile>\<^sub>t P {c\<^sub>1} P'" using m(1) conseq by auto
+    hence c1: "R,G \<turnstile>\<^sub>t P {c\<^sub>1} P'" using m(1) conseq by auto
     show ?case 
     proof (rule Seq(1)[OF _ c1 outer(2) \<alpha>(1) i(1)], goal_cases inner)
       case (inner P'' M'')
@@ -179,40 +168,40 @@ next
 next
   case (Choice c\<^sub>1 c\<^sub>2)
   hence \<alpha>: "\<alpha>' < c\<^sub>1 <\<^sub>p \<alpha>" "\<alpha>' < c\<^sub>2 <\<^sub>p \<alpha>" by auto
-  obtain m: "R,G,X \<turnstile>\<^sub>t P {c\<^sub>1} M" "R,G,X \<turnstile>\<^sub>t P {c\<^sub>2} M" using Choice(4) by blast
-  have i: "inter\<^sub>c R G X c\<^sub>1 \<alpha>" "inter\<^sub>c R G X c\<^sub>2 \<alpha>" using Choice by auto
+  obtain m: "R,G \<turnstile>\<^sub>t P {c\<^sub>1} M" "R,G \<turnstile>\<^sub>t P {c\<^sub>2} M" using Choice(4) by blast
+  have i: "inter\<^sub>c R G c\<^sub>1 \<alpha>" "inter\<^sub>c R G c\<^sub>2 \<alpha>" using Choice by auto
   show ?case
   proof (rule Choice(2)[OF _ m(2) Choice(5) \<alpha>(2) i(2)], goal_cases outer)
     case (outer P' N')
     show ?case 
     proof (rule Choice(1)[OF _ m(1) Choice(5) \<alpha>(1) i (1)], goal_cases inner)
       case (inner P'' N'')
-      hence "R,G,X \<turnstile>\<^sub>t (N' \<inter> N'') {c\<^sub>1} Q"
+      hence "R,G \<turnstile>\<^sub>t (N' \<inter> N'') {c\<^sub>1} Q"
         using outer by (meson Int_lower2 subset_refl lrules.conseq)
-      moreover have "R,G,X \<turnstile>\<^sub>t (N' \<inter> N'') {c\<^sub>2} Q" 
+      moreover have "R,G \<turnstile>\<^sub>t (N' \<inter> N'') {c\<^sub>2} Q" 
         using inner outer by (meson Int_lower1 subset_refl lrules.conseq)
-      ultimately have "R,G,X \<turnstile>\<^sub>t (N' \<inter> N'') {c\<^sub>1 \<sqinter> c\<^sub>2} Q" by auto
+      ultimately have "R,G \<turnstile>\<^sub>t (N' \<inter> N'') {c\<^sub>1 \<sqinter> c\<^sub>2} Q" by auto
       moreover have "P \<subseteq> P' \<inter> P''" using outer inner by auto
       ultimately show ?case using actomic_conjI[OF outer(2) inner(2)] Choice(3) by blast 
     qed
   qed
 next
   case (Loop c)
-  then obtain I where i: "P \<subseteq> I" "R,G,X \<turnstile>\<^sub>t I {c} I" "stable R I" "I \<subseteq> M" by auto
+  then obtain I where i: "P \<subseteq> I" "R,G \<turnstile>\<^sub>t I {c} I" "stable R I" "I \<subseteq> M" by auto
   have [simp]: "\<alpha>' = \<alpha>" using Loop by auto
   have \<alpha>: "\<alpha> < c <\<^sub>p \<alpha>" using Loop by auto
-  have "R,G,X \<turnstile>\<^sub>A I {\<alpha>} Q" using Loop(4) i(3,4) by (meson atomic_pre)
-  hence s: "R,G,X \<turnstile>\<^sub>A I {\<alpha>} (sp \<alpha> R I)" "sp \<alpha> R I \<subseteq> Q" using atomic_strongest by auto
-  have d: "inter\<^sub>c R G X c \<alpha>" using Loop by auto
+  have "R,G \<turnstile>\<^sub>A I {\<alpha>} Q" using Loop(4) i(3,4) by (meson atomic_pre)
+  hence s: "R,G \<turnstile>\<^sub>A I {\<alpha>} (sp \<alpha> R I)" "sp \<alpha> R I \<subseteq> Q" using atomic_strongest by auto
+  have d: "inter\<^sub>c R G c \<alpha>" using Loop by auto
 
   show ?case
   proof (rule Loop(1)[OF _ i(2) s(1) \<alpha> d], goal_cases outer)
     case (outer P' I')
-    hence "R,G,X \<turnstile>\<^sub>A I {\<alpha>} I'" using i(3) by (meson atomic_pre)
+    hence "R,G \<turnstile>\<^sub>A I {\<alpha>} I'" using i(3) by (meson atomic_pre)
     hence "sp \<alpha> R I \<subseteq> I'" using atomic_strongest by auto
-    hence "R,G,X \<turnstile>\<^sub>t (sp \<alpha> R I) {c} (sp \<alpha> R I)" using outer(3) lrules.conseq by simp
-    hence "R,G,X \<turnstile>\<^sub>t (sp \<alpha> R I) {c*} (sp \<alpha> R I)" using s(1) by (meson loop atomic_rule_def)
-    hence "R,G,X \<turnstile>\<^sub>t (sp \<alpha> R I) {c*} Q" using s(2) conseq by blast
+    hence "R,G \<turnstile>\<^sub>t (sp \<alpha> R I) {c} (sp \<alpha> R I)" using outer(3) lrules.conseq by simp
+    hence "R,G \<turnstile>\<^sub>t (sp \<alpha> R I) {c*} (sp \<alpha> R I)" using s(1) by (meson loop atomic_rule_def)
+    hence "R,G \<turnstile>\<^sub>t (sp \<alpha> R I) {c*} Q" using s(2) conseq by blast
     then show ?case using Loop(2)[OF i(1)] s(1) by simp
   qed
 qed auto
@@ -221,105 +210,105 @@ section \<open>Transition Rules\<close>
 
 text \<open>Local judgements are preserved across silent steps\<close>
 lemma rewriteI [intro]:
-  assumes "R,G,X \<turnstile>\<^sub>t P {c} Q"
+  assumes "R,G \<turnstile>\<^sub>t P {c} Q"
   assumes "c \<leadsto> c'"
-  shows "R,G,X \<turnstile>\<^sub>t P {c'} Q"
+  shows "R,G \<turnstile>\<^sub>t P {c'} Q"
   using assms
 proof (induct arbitrary: c' rule: lrules.induct)
-  case (seq R G X P c\<^sub>1 Q c\<^sub>2 M)
+  case (seq R G P c\<^sub>1 Q c\<^sub>2 M)
   show ?case using seq(5,1,2,3,4) by cases blast+
 next
-  case (loop R P G X c)
+  case (loop R P G c)
   thus ?case by cases blast+
 qed auto
 
 text \<open>Global judgements are preserved across silent steps\<close>
 lemma g_rewriteI [intro]:
-  assumes "R,G,X \<turnstile> P {c} Q"
+  assumes "R,G \<turnstile> P {c} Q"
   assumes "c \<leadsto> c'"
-  shows "R,G,X \<turnstile> P {c'} Q"
+  shows "R,G \<turnstile> P {c'} Q"
   using assms
 proof (induct arbitrary: c' rule: rules.induct)
-  case (par R\<^sub>1 G\<^sub>1 X P\<^sub>1 c\<^sub>1 Q\<^sub>1 R\<^sub>2 G\<^sub>2 P\<^sub>2 c\<^sub>2 Q\<^sub>2)
-  show ?case using par(7,1,2,3,4,5,6) by cases blast+
+  case (par R\<^sub>1 G\<^sub>1 P\<^sub>1 c\<^sub>1 Q\<^sub>1 R\<^sub>2 G\<^sub>2 P\<^sub>2 c\<^sub>2 Q\<^sub>2)
+  show ?case using par(7,1,2,3,4,5,6) by (cases) blast+
 qed auto
 
 text \<open>Local judgements are preserved across execution steps\<close>
 lemma stepI:
-  assumes "c \<mapsto>[\<alpha>,r,\<alpha>'] c'" "R,G,X \<turnstile>\<^sub>t P {c} Q"
-  assumes "inter\<^sub>c R G X r \<alpha>'"
-  shows "\<exists>P' M. P \<subseteq> P' \<and> (R,G,X \<turnstile>\<^sub>A P' {\<alpha>} M) \<and> (R,G,X \<turnstile>\<^sub>t M {c'} Q)"
+  assumes "c \<mapsto>[\<alpha>,r,\<alpha>'] c'" "R,G \<turnstile>\<^sub>t P {c} Q"
+  assumes "inter\<^sub>c R G r \<alpha>'"
+  shows "\<exists>P' M. P \<subseteq> P' \<and> (R,G \<turnstile>\<^sub>A P' {\<alpha>} M) \<and> (R,G \<turnstile>\<^sub>t M {c'} Q)"
   using assms
-proof (induct arbitrary: P R G X Q)
+proof (induct arbitrary: P R G Q)
   case (act \<alpha>)
   then show ?case by (elim basicE) (meson atomic_rule_def nil lrules.conseq order_refl)
 next
   case (pre c\<^sub>1 \<alpha> c \<alpha>' c\<^sub>1' c\<^sub>2)
-  obtain M' where m: "R,G,X \<turnstile>\<^sub>t P {c\<^sub>1} M'" "R,G,X \<turnstile>\<^sub>t M' {c\<^sub>2} Q" using pre by fast
+  obtain M' where m: "R,G \<turnstile>\<^sub>t P {c\<^sub>1} M'" "R,G \<turnstile>\<^sub>t M' {c\<^sub>2} Q" using pre by fast
   then show ?case using pre(2)[OF m(1) pre(4)] m(2) by blast
 next
   case (pst c\<^sub>2 \<alpha> c \<alpha>' c\<^sub>2' \<gamma> c\<^sub>1)
-  obtain M' where m: "R,G,X \<turnstile>\<^sub>t P {c\<^sub>1} M'" "R,G,X \<turnstile>\<^sub>t M' {c\<^sub>2} Q" using pst by fast
-  have i: "inter\<^sub>c R G X c\<^sub>1 (fwd_prog \<alpha>' c)" "inter\<^sub>c R G X c \<alpha>'" using pst by auto
-  obtain P' M where m': "M' \<subseteq> P'" "R,G,X \<turnstile>\<^sub>A P' {\<alpha>} M" "R,G,X \<turnstile>\<^sub>t M {c\<^sub>2'} Q"
+  obtain M' where m: "R,G \<turnstile>\<^sub>t P {c\<^sub>1} M'" "R,G \<turnstile>\<^sub>t M' {c\<^sub>2} Q" using pst by fast
+  have i: "inter\<^sub>c R G c\<^sub>1 (fwd_prog \<alpha>' c)" "inter\<^sub>c R G c \<alpha>'" using pst by auto
+  obtain P' M where m': "M' \<subseteq> P'" "R,G \<turnstile>\<^sub>A P' {\<alpha>} M" "R,G \<turnstile>\<^sub>t M {c\<^sub>2'} Q"
     using pst(2)[OF m(2) i(2)] by blast
-  hence m'': "R,G,X \<turnstile>\<^sub>t P {c\<^sub>1} P'" using m(1) by blast
+  hence m'': "R,G \<turnstile>\<^sub>t P {c\<^sub>1} P'" using m(1) by blast
   have "fwd_prog \<alpha>' c = \<alpha>" using pst(1) collect_reorder by auto
   then show ?case using reorder_prog[OF m'' m'(2) pst(3)] i(1) m'(3) by (metis seq)
 qed 
 
 text \<open>Global judgements are preserved across execution steps\<close>
 lemma g_stepI:
-  assumes "R,G,X \<turnstile> P {c} Q"
+  assumes "R,G \<turnstile> P {c} Q"
   assumes "c \<mapsto>\<^sub>\<alpha> c'"
-  shows "\<exists>P' M. P \<subseteq> P' \<and> (R,G,X \<turnstile>\<^sub>A P' {\<alpha>} M) \<and> (R,G,X \<turnstile> M {c'} Q)"
+  shows "\<exists>P' M. P \<subseteq> P' \<and> (R,G \<turnstile>\<^sub>A P' {\<alpha>} M) \<and> (R,G \<turnstile> M {c'} Q)"
   using assms
 proof (induct arbitrary: \<alpha> c' rule: rules.induct)
-  case (par R\<^sub>1 G\<^sub>1 X P\<^sub>1 c\<^sub>1 Q\<^sub>1 R\<^sub>2 G\<^sub>2 P\<^sub>2 c\<^sub>2 Q\<^sub>2)
+  case (par R\<^sub>1 G\<^sub>1 P\<^sub>1 c\<^sub>1 Q\<^sub>1 R\<^sub>2 G\<^sub>2 P\<^sub>2 c\<^sub>2 Q\<^sub>2)
   show ?case using par(7)
   proof cases
     case (par1 c\<^sub>1')
-    obtain M\<^sub>2 where m2: "P\<^sub>2 \<subseteq> M\<^sub>2" "stable R\<^sub>2 M\<^sub>2" "R\<^sub>2,G\<^sub>2,X \<turnstile> M\<^sub>2 {c\<^sub>2} Q\<^sub>2" using par
+    obtain M\<^sub>2 where m2: "P\<^sub>2 \<subseteq> M\<^sub>2" "stable R\<^sub>2 M\<^sub>2" "R\<^sub>2,G\<^sub>2 \<turnstile> M\<^sub>2 {c\<^sub>2} Q\<^sub>2" using par
       by (meson g_stable_preE)
-    obtain P M\<^sub>1 where m1: "P\<^sub>1 \<subseteq> P" "R\<^sub>1,G\<^sub>1,X \<turnstile>\<^sub>A P { \<alpha> } M\<^sub>1" "R\<^sub>1,G\<^sub>1,X \<turnstile> M\<^sub>1 {c\<^sub>1'} Q\<^sub>1" 
+    obtain P M\<^sub>1 where m1: "P\<^sub>1 \<subseteq> P" "R\<^sub>1,G\<^sub>1 \<turnstile>\<^sub>A P { \<alpha> } M\<^sub>1" "R\<^sub>1,G\<^sub>1 \<turnstile> M\<^sub>1 {c\<^sub>1'} Q\<^sub>1" 
       using par1 par(2)[OF par1(2)] by blast
-    hence "R\<^sub>1 \<inter> R\<^sub>2,G\<^sub>1 \<union> G\<^sub>2,X \<turnstile> M\<^sub>1 \<inter> M\<^sub>2 {c'} Q\<^sub>1 \<inter> Q\<^sub>2" using par1 m2 par by blast
-    moreover have "R\<^sub>1 \<inter> R\<^sub>2,G\<^sub>1 \<union> G\<^sub>2,X \<turnstile>\<^sub>A P \<inter> M\<^sub>2 { \<alpha> } M\<^sub>1 \<inter> M\<^sub>2" 
+    hence "R\<^sub>1 \<inter> R\<^sub>2,G\<^sub>1 \<union> G\<^sub>2 \<turnstile> M\<^sub>1 \<inter> M\<^sub>2 {c'} Q\<^sub>1 \<inter> Q\<^sub>2" using par1 m2 par by blast
+    moreover have "R\<^sub>1 \<inter> R\<^sub>2,G\<^sub>1 \<union> G\<^sub>2 \<turnstile>\<^sub>A P \<inter> M\<^sub>2 { \<alpha> } M\<^sub>1 \<inter> M\<^sub>2" 
       using m1(2) m2(2) par.hyps(6) by blast
     ultimately show ?thesis using m2(1) m1(1) by blast
   next
     case (par2 c\<^sub>2')
-    obtain M\<^sub>1 where m1: "P\<^sub>1 \<subseteq> M\<^sub>1" "stable R\<^sub>1 M\<^sub>1" "R\<^sub>1,G\<^sub>1,X \<turnstile> M\<^sub>1 {c\<^sub>1} Q\<^sub>1" using par
+    obtain M\<^sub>1 where m1: "P\<^sub>1 \<subseteq> M\<^sub>1" "stable R\<^sub>1 M\<^sub>1" "R\<^sub>1,G\<^sub>1 \<turnstile> M\<^sub>1 {c\<^sub>1} Q\<^sub>1" using par
       by (meson g_stable_preE)
-    obtain P M\<^sub>2 where m2: "P\<^sub>2 \<subseteq> P" "R\<^sub>2,G\<^sub>2,X \<turnstile>\<^sub>A P { \<alpha> } M\<^sub>2" "R\<^sub>2,G\<^sub>2,X \<turnstile> M\<^sub>2 {c\<^sub>2'} Q\<^sub>2"
+    obtain P M\<^sub>2 where m2: "P\<^sub>2 \<subseteq> P" "R\<^sub>2,G\<^sub>2 \<turnstile>\<^sub>A P { \<alpha> } M\<^sub>2" "R\<^sub>2,G\<^sub>2 \<turnstile> M\<^sub>2 {c\<^sub>2'} Q\<^sub>2"
       using par2 par(4)[OF par2(2)] by blast
-    hence "R\<^sub>1 \<inter> R\<^sub>2,G\<^sub>1 \<union> G\<^sub>2,X \<turnstile> M\<^sub>1 \<inter> M\<^sub>2 {c'} Q\<^sub>1 \<inter> Q\<^sub>2" using par2 m1 par by blast
-    moreover have "R\<^sub>2 \<inter> R\<^sub>1,G\<^sub>1 \<union> G\<^sub>2,X \<turnstile>\<^sub>A P \<inter> M\<^sub>1 { \<alpha> } M\<^sub>2 \<inter> M\<^sub>1" 
+    hence "R\<^sub>1 \<inter> R\<^sub>2,G\<^sub>1 \<union> G\<^sub>2 \<turnstile> M\<^sub>1 \<inter> M\<^sub>2 {c'} Q\<^sub>1 \<inter> Q\<^sub>2" using par2 m1 par by blast
+    moreover have "R\<^sub>2 \<inter> R\<^sub>1,G\<^sub>1 \<union> G\<^sub>2 \<turnstile>\<^sub>A P \<inter> M\<^sub>1 { \<alpha> } M\<^sub>2 \<inter> M\<^sub>1" 
       using atomic_frameI[OF m2(2) m1(2) par(5)] by blast
     ultimately show ?thesis using m2(1) m1(1) by (metis inf_commute inf_mono)
   qed 
 next
-  case (conseq R G X P c Q P' R' G' Q')
+  case (conseq R G P c Q P' R' G' Q')
   thus ?case using rules.conseq atomic_conseqI by (meson order_refl subset_trans)
 next
-  case (frame R G X P c Q R' M')
-  then obtain P' M where "P \<subseteq> P'" "R,G,X \<turnstile>\<^sub>A P' {\<alpha>} M" "R,G,X \<turnstile> M {c'} Q" by metis
+  case (frame R G P c Q R' M')
+  then obtain P' M where "P \<subseteq> P'" "R,G \<turnstile>\<^sub>A P' {\<alpha>} M" "R,G \<turnstile> M {c'} Q" by metis
   thus ?case using rules.frame atomic_frameI frame(3,4) by blast
 next
-  case (thread R G X P c Q)
+  case (thread R G P c Q)
   hence "local_only c" using thread_only by auto
   then obtain r \<alpha>'' where c: "c \<mapsto>[\<alpha>,r,\<alpha>''] c'" using thread exec_collect by blast
   then show ?case 
     using stepI[OF c thread(1)] thread(2) indep_stepI[OF thread(2) c] by auto 
 qed
 
-section \<open>Theorem\<close>
+section \<open>Sound Transition Theorem\<close>
 
 text \<open>All transitions that start with a program with a logic judgement and satisfy
       the precondition and environment rely should conform to the guarantee and
       establish the postcondition if they terminate\<close>
 lemma sound_transitions:
-  assumes "t \<in> transitions" "fst (t ! 0) = c" "R,G,X \<turnstile> P {c} Q" "t \<in> pre P \<inter> rely R"
+  assumes "t \<in> transitions" "fst (t ! 0) = c" "R,G \<turnstile> P {c} Q" "t \<in> pre P \<inter> rely R"
   shows "t \<in> guar G \<inter> post Q"
   using assms
 proof (induct arbitrary: c P rule: transitions.induct)
@@ -327,12 +316,12 @@ proof (induct arbitrary: c P rule: transitions.induct)
   thus ?case using guar_def by force
 next
   case (env s s' t)
-  then obtain P' where "P \<subseteq> P'" "stable R P'" "R,G,X \<turnstile> P' {c} Q" by (metis g_stable_preE) 
+  then obtain P' where "P \<subseteq> P'" "stable R P'" "R,G \<turnstile> P' {c} Q" by (metis g_stable_preE) 
   thus ?case using env by (auto simp: stable_def)
 next
   case (prg s s' t)
   then obtain \<alpha> where \<alpha>: "c \<mapsto>\<^sub>\<alpha> (fst s')" "(snd s,snd s') \<in> eval \<alpha>" by auto
-  then obtain P' M where "P \<subseteq> P'" "R,G,X \<turnstile>\<^sub>A P' {\<alpha>} M" "R,G,X \<turnstile> M {fst s'} Q"
+  then obtain P' M where "P \<subseteq> P'" "R,G \<turnstile>\<^sub>A P' {\<alpha>} M" "R,G \<turnstile> M {fst s'} Q"
     using g_stepI[OF prg(5) \<alpha>(1)] by metis
   thus ?case using prg \<alpha> unfolding atomic_rule_def wp_def spec_def by fastforce
 next
@@ -342,7 +331,7 @@ qed
 
 text \<open>Soundness Theorem\<close>
 theorem sound:
-  assumes "R,G,X \<turnstile> P { c } Q"
+  assumes "R,G \<turnstile> P { c } Q"
   shows "\<Turnstile> c SAT [P, R, G, Q]"
   using assms sound_transitions by (auto simp: validity_def cp_def)
 
