Syntax.thy
@@ -1,0 +1,17 @@
+theory Syntax
+  imports Main
+begin
+
+chapter \<open>Syntax\<close>
+
+text \<open>Basic While Language syntax, with parallel composition\<close>
+
+datatype 'a com =
+  Nil
+  | Basic "'a"
+  | Seq "'a com" "'a com" (infixr ";" 80)
+  | Choice "'a com" "'a com" (infixr "\<sqinter>" 150)
+  | Loop "'a com" ("_*" [100] 150)
+  | Parallel "'a com" "'a com"  (infixr "||" 150)
+
+end
